Weidenbach_Book/CDCL_W_Restart.thy
@@ -6,6 +6,7 @@ subsection \<open>Adding Restarts\<close>
 locale cdcl\<^sub>W_restart_restart =
   conflict_driven_clause_learning\<^sub>W
     state_eq
+    state
     \<comment> \<open>functions for the state: \<close>
       \<comment> \<open>access functions:\<close>
     trail init_clss learned_clss backtrack_lvl conflicting
@@ -17,6 +18,8 @@ locale cdcl\<^sub>W_restart_restart =
     init_state
   for
     state_eq :: "'st \<Rightarrow> 'st \<Rightarrow> bool" (infix "\<sim>" 50) and
+    state :: "'st \<Rightarrow> ('v, 'v clause) ann_lits \<times> 'v clauses \<times> 'v clauses \<times> nat \<times> 'v clause option \<times>
+      'b" and
     trail :: "'st \<Rightarrow> ('v, 'v clause) ann_lits" and
     init_clss :: "'st \<Rightarrow> 'v clauses" and
     learned_clss :: "'st \<Rightarrow> 'v clauses" and
@@ -535,7 +538,7 @@ locale luby_sequence_restart =
   luby_sequence ur +
   conflict_driven_clause_learning\<^sub>W
     \<comment> \<open>functions for the state: \<close>
-    state_eq
+    state_eq state
       \<comment> \<open>access functions:\<close>
     trail init_clss learned_clss backtrack_lvl conflicting
       \<comment> \<open>changing state:\<close>
@@ -547,6 +550,8 @@ locale luby_sequence_restart =
   for
     ur :: nat and
     state_eq :: "'st \<Rightarrow> 'st \<Rightarrow> bool" (infix "\<sim>" 50) and
+    state :: "'st \<Rightarrow> ('v, 'v clause) ann_lits \<times> 'v clauses \<times> 'v clauses \<times> nat \<times> 'v clause option \<times>
+      'b" and
     trail :: "'st \<Rightarrow> ('v, 'v clause) ann_lits" and
     hd_trail :: "'st \<Rightarrow> ('v, 'v clause) ann_lit" and
     init_clss :: "'st \<Rightarrow> 'v clauses" and
